src/DY.Example.NSL.Protocol.Stateful.Proof.fst
@@ -59,13 +59,13 @@ let nsl_trace_invs: trace_invariants (nsl_crypto_invs) = {
       match parse nsl_event evt with
       | Some (Initiate1 alice bob n_a) -> (
         prin == alice /\
-        get_label n_a == join (principal_label alice) (principal_label bob) /\
+        get_label nsl_crypto_usages n_a == join (principal_label alice) (principal_label bob) /\
         0 < DY.Core.Trace.Type.length tr /\
         rand_generated_at tr (DY.Core.Trace.Type.length tr - 1) n_a
       )
       | Some (Respond1 alice bob n_a n_b) -> (
         prin == bob /\
-        get_label n_b == join (principal_label alice) (principal_label bob) /\
+        get_label nsl_crypto_usages n_b == join (principal_label alice) (principal_label bob) /\
         0 < DY.Core.Trace.Type.length tr /\
         rand_generated_at tr (DY.Core.Trace.Type.length tr - 1) n_b
       )
@@ -154,8 +154,8 @@ let send_msg1_proof tr global_sess_id alice sess_id =
   | Some msg_id -> (
     let (Some (InitiatorSentMsg1 bob n_a), tr) = get_typed_state #nsl_session nsl_session_label alice sess_id tr in
     let (Some (pk_b, nonce), tr) = (
-      let*? pk_b = get_public_key alice global_sess_id.pki PkEnc bob in
-      let* nonce = mk_rand (principal_label alice) 32 in
+      let*? pk_b = get_public_key alice global_sess_id.pki (PkEnc "NSL.PublicKey") bob in
+      let* nonce = mk_rand Unknown (principal_label alice) 32 in
       return (Some (pk_b, nonce))
     ) tr in
     compute_message1_proof tr alice bob pk_b n_a nonce
@@ -179,7 +179,7 @@ let prepare_msg2_proof tr global_sess_id bob msg_id =
   | Some sess_id -> (
     let (Some (msg, sk_b, msg1), tr) = (
       let*? msg = recv_msg msg_id in
-      let*? sk_b = get_private_key bob global_sess_id.private_keys PkDec in
+      let*? sk_b = get_private_key bob global_sess_id.private_keys (PkDec "NSL.PublicKey") in
       let*? msg1: message1 = return (decode_message1 bob msg sk_b) in
       return (Some (msg, sk_b, msg1))
     ) tr in
@@ -205,8 +205,8 @@ let send_msg2_proof tr global_sess_id bob sess_id =
   | Some msg_id -> (
     let (Some (ResponderSentMsg2 alice n_a n_b), tr) = get_typed_state #nsl_session nsl_session_label bob sess_id tr in
     let (Some (pk_a, nonce), tr) = (
-      let*? pk_a = get_public_key bob global_sess_id.pki PkEnc alice in
-      let* nonce = mk_rand (principal_label bob) 32 in
+      let*? pk_a = get_public_key bob global_sess_id.pki (PkEnc "NSL.PublicKey") alice in
+      let* nonce = mk_rand Unknown (principal_label bob) 32 in
       return (Some (pk_a, nonce))
     ) tr in
     let msg = compute_message2 bob {n_a; alice;} pk_a n_b nonce in
@@ -231,7 +231,7 @@ let prepare_msg3_proof tr global_sess_id alice sess_id msg_id =
   | Some _ -> (
     let (Some (msg, sk_a, InitiatorSentMsg1 bob n_a), tr) = (
       let*? msg = recv_msg msg_id in
-      let*? sk_a = get_private_key alice global_sess_id.private_keys PkDec in
+      let*? sk_a = get_private_key alice global_sess_id.private_keys (PkDec "NSL.PublicKey") in
       let*? st: nsl_session = get_typed_state nsl_session_label alice sess_id in
       return (Some (msg, sk_a, st))
     ) tr in
@@ -260,8 +260,8 @@ let send_msg3_proof tr global_sess_id alice sess_id =
   | Some msg_id -> (
     let (Some (InitiatorSentMsg3 bob n_a n_b), tr) = get_typed_state #nsl_session nsl_session_label alice sess_id tr in
     let (Some (pk_b, nonce), tr) = (
-      let*? pk_b = get_public_key alice global_sess_id.pki PkEnc bob in
-      let* nonce = mk_rand (principal_label alice) 32 in
+      let*? pk_b = get_public_key alice global_sess_id.pki (PkEnc "NSL.PublicKey") bob in
+      let* nonce = mk_rand Unknown (principal_label alice) 32 in
       return (Some (pk_b, nonce))
     ) tr in
     let msg = compute_message3 alice bob pk_b n_b nonce in
@@ -304,7 +304,7 @@ let prepare_msg4 tr global_sess_id bob sess_id msg_id =
   | Some _ -> (
     let (Some (msg, sk_b, ResponderSentMsg2 alice n_a n_b), tr) = (
       let*? msg = recv_msg msg_id in
-      let*? sk_b = get_private_key bob global_sess_id.private_keys PkDec in
+      let*? sk_b = get_private_key bob global_sess_id.private_keys (PkDec "NSL.PublicKey") in
       let*? st: nsl_session = get_typed_state nsl_session_label bob sess_id in
       return (Some (msg, sk_b, st))
     ) tr in
@@ -333,8 +333,8 @@ let prepare_msg4 tr global_sess_id bob sess_id msg_id =
     let msg3: message3 = msg3 in
 
     introduce (~((join (principal_label alice) (principal_label bob)) `can_flow tr` public)) ==> event_triggered tr alice nsl_event_label (serialize nsl_event (Initiate2 alice bob n_a n_b)) with _. (
-      assert(exists alice' n_a'. get_label n_b `can_flow tr` (principal_label alice') /\ event_triggered tr alice' nsl_event_label (serialize nsl_event #(nsl_event_parseable_serializeable bytes) (Initiate2 alice' bob n_a' n_b)));
-      eliminate exists alice' n_a'. get_label n_b `can_flow tr` (principal_label alice') /\ event_triggered tr alice' nsl_event_label (serialize nsl_event #(nsl_event_parseable_serializeable bytes) (Initiate2 alice' bob n_a' n_b))
+      assert(exists alice' n_a'. get_label nsl_crypto_usages n_b `can_flow tr` (principal_label alice') /\ event_triggered tr alice' nsl_event_label (serialize nsl_event #(nsl_event_parseable_serializeable bytes) (Initiate2 alice' bob n_a' n_b)));
+      eliminate exists alice' n_a'. get_label nsl_crypto_usages n_b `can_flow tr` (principal_label alice') /\ event_triggered tr alice' nsl_event_label (serialize nsl_event #(nsl_event_parseable_serializeable bytes) (Initiate2 alice' bob n_a' n_b))
       returns _
       with _. (
         event_respond1_injective tr alice alice' bob n_a n_a' n_b
