src/DY.Example.NSL.Protocol.Stateful.fst
@@ -46,7 +46,7 @@ type nsl_global_sess_ids = {
 
 val prepare_msg1: principal -> principal -> crypto nat
 let prepare_msg1 alice bob =
-  let* n_a = mk_rand (join (principal_label alice) (principal_label bob)) 32 in
+  let* n_a = mk_rand Unknown (join (principal_label alice) (principal_label bob)) 32 in
   trigger_event alice nsl_event_label (serialize nsl_event (Initiate1 alice bob n_a));*
   let* sess_id = new_session_id alice in
   set_typed_state nsl_session_label alice sess_id (InitiatorSentMsg1 bob n_a <: nsl_session);*
@@ -57,8 +57,8 @@ let send_msg1 global_sess_id alice sess_id =
   let*? st: nsl_session = get_typed_state nsl_session_label alice sess_id in
   match st with
   | InitiatorSentMsg1 bob n_a -> (
-    let*? pk_b = get_public_key alice global_sess_id.pki PkEnc bob in
-    let* nonce = mk_rand (principal_label alice) 32 in
+    let*? pk_b = get_public_key alice global_sess_id.pki (PkEnc "NSL.PublicKey") bob in
+    let* nonce = mk_rand Unknown (principal_label alice) 32 in
     let msg = compute_message1 alice bob pk_b n_a nonce in
     let* msg_id = send_msg msg in
     return (Some msg_id)
@@ -68,9 +68,9 @@ let send_msg1 global_sess_id alice sess_id =
 val prepare_msg2: nsl_global_sess_ids -> principal -> nat -> crypto (option nat)
 let prepare_msg2 global_sess_id bob msg_id =
   let*? msg = recv_msg msg_id in
-  let*? sk_b = get_private_key bob global_sess_id.private_keys PkDec in
+  let*? sk_b = get_private_key bob global_sess_id.private_keys (PkDec "NSL.PublicKey") in
   let*? msg1: message1 = return (decode_message1 bob msg sk_b) in
-  let* n_b = mk_rand (join (principal_label msg1.alice) (principal_label bob)) 32 in
+  let* n_b = mk_rand Unknown (join (principal_label msg1.alice) (principal_label bob)) 32 in
   trigger_event bob nsl_event_label (serialize nsl_event (Respond1 msg1.alice bob msg1.n_a n_b));*
   let* sess_id = new_session_id bob in
   set_typed_state nsl_session_label bob sess_id (ResponderSentMsg2 msg1.alice msg1.n_a n_b <: nsl_session);*
@@ -81,8 +81,8 @@ let send_msg2 global_sess_id bob sess_id =
   let*? st: nsl_session = get_typed_state nsl_session_label bob sess_id in
   match st with
   | ResponderSentMsg2 alice n_a n_b -> (
-    let*? pk_a = get_public_key bob global_sess_id.pki PkEnc alice in
-    let* nonce = mk_rand (principal_label bob) 32 in
+    let*? pk_a = get_public_key bob global_sess_id.pki (PkEnc "NSL.PublicKey") alice in
+    let* nonce = mk_rand Unknown (principal_label bob) 32 in
     let msg = compute_message2 bob {n_a; alice;} pk_a n_b nonce in
     let* msg_id = send_msg msg in
     return (Some msg_id)
@@ -92,7 +92,7 @@ let send_msg2 global_sess_id bob sess_id =
 val prepare_msg3: nsl_global_sess_ids -> principal -> nat -> nat -> crypto (option unit)
 let prepare_msg3 global_sess_id alice sess_id msg_id =
   let*? msg = recv_msg msg_id in
-  let*? sk_a = get_private_key alice global_sess_id.private_keys PkDec in
+  let*? sk_a = get_private_key alice global_sess_id.private_keys (PkDec "NSL.PublicKey") in
   let*? st: nsl_session = get_typed_state nsl_session_label alice sess_id in
   match st with
   | InitiatorSentMsg1 bob n_a -> (
@@ -108,8 +108,8 @@ let send_msg3 global_sess_id alice sess_id =
   let*? st: nsl_session = get_typed_state nsl_session_label alice sess_id in
   match st with
   | InitiatorSentMsg3 bob n_a n_b -> (
-    let*? pk_b = get_public_key alice global_sess_id.pki PkEnc bob in
-    let* nonce = mk_rand (principal_label alice) 32 in
+    let*? pk_b = get_public_key alice global_sess_id.pki (PkEnc "NSL.PublicKey") bob in
+    let* nonce = mk_rand Unknown (principal_label alice) 32 in
     let msg = compute_message3 alice bob pk_b n_b nonce in
     let* msg_id = send_msg msg in
     return (Some msg_id)
@@ -119,7 +119,7 @@ let send_msg3 global_sess_id alice sess_id =
 val prepare_msg4: nsl_global_sess_ids -> principal -> nat -> nat -> crypto (option unit)
 let prepare_msg4 global_sess_id bob sess_id msg_id =
   let*? msg = recv_msg msg_id in
-  let*? sk_b = get_private_key bob global_sess_id.private_keys PkDec in
+  let*? sk_b = get_private_key bob global_sess_id.private_keys (PkDec "NSL.PublicKey") in
   let*? st: nsl_session = get_typed_state nsl_session_label bob sess_id in
   match st with
   | ResponderSentMsg2 alice n_a n_b -> (
